stash attempt -- not working

src/vector.ml
@@ -1,0 +1,88 @@
+let length l = 
+  CCVector.size l
+
+let app l1 l2 = 
+  let l = CCVector.copy l1 in 
+  CCVector.iter (CCVector.push l) l2; l
+
+let nth_error l n =
+  try Some (CCVector.get l n)
+  with | _ -> None
+
+let nth n l d = 
+  try CCVector.get l n
+  with | _ -> d
+
+let rev l = 
+  CCVector.rev l
+
+let in_dec eqb x l = 
+  CCVector.member ~eq:eqb x l
+
+let vec_eq_dec eqb l1 l2 = 
+  CCVector.equal eqb l1 l2
+
+let flatten vv = 
+  let result = CCVector.create () in
+  CCVector.iter
+    (fun inner_vec ->
+       CCVector.iter (fun x -> CCVector.push result x) inner_vec
+    )
+    vv;
+  result
+
+let map f l = 
+  CCVector.map f l
+
+let fold_left f l init =
+  CCVector.fold f init l
+
+let forallb f l = 
+  let bs = map f l in 
+  fold_left (&&) bs true
+
+let combine l1 l2 =
+  CCVector.monoid_product (,) l1 l2
+
+let slice l start len =
+  let result = CCVector.create () in
+  CCVector.slice_iter v start len (fun x -> CCVector.push result x);
+  result
+
+let firstn n l = 
+  slice l 0 n
+
+let skipn n l = 
+  let len = length l in
+  if n < length l then
+    slice l n (length l - n)
+  else 
+    CCVector.create ()
+    
+let nodup eqb l = 
+  let result = CCVector.create () in
+  CCVector.iter (fun x -> if not (in_dec eqb x l) then CCVector.push result x) l;
+  result
+
+let repeat x n = 
+  CCVector.make n x
+
+let rcons l x = 
+  let l' = CCVector.copy l in
+  CCVector.push l x;
+  l
+
+let unrcons l = 
+  let len = length l in 
+  if len = 0 then None
+  else Some (firstn (len-1) l, CCVector.get l (len-1))
+
+(* Very inefficient *)
+let set_nth x l n y =
+  let len = length l in
+  if n < len then
+    let l' = CCVector.copy l in 
+      CCVector.set l' n y;
+      l'
+  else
+    rcons (app l (repeat x (len - n))) y
