src/vector.mli
@@ -1,0 +1,33 @@
+open CCVector
+
+val length : 'a vector -> int
+
+val app : 'a vector -> 'a vector -> 'a vector
+
+val nth_error : 'a vector -> int -> 'a option
+
+val nth : int -> 'a vector -> 'a -> 'a
+
+val rev : 'a vector -> 'a vector
+
+val in_dec : ('a -> 'a -> bool) -> 'a -> 'a vector -> bool
+
+val vec_eq_dec : ('a -> 'a -> bool) -> 'a vector -> 'a vector -> bool
+
+val flatten : ('a vector) vector -> 'a vector
+
+val map : ('a -> 'b) -> 'a vector -> 'b vector
+
+val firstn : 'a vector -> int -> 'a vector
+
+val skipn : 'a vector -> int -> 'a vector
+
+val nodup : ('a -> 'a -> bool) -> 'a vector -> 'a vector
+
+val repeat : int -> 'a -> 'a vector
+
+val rcons : 'a vector -> 'a -> 'a vector
+
+val unrcons : 'a vector -> ('a vector * 'a) option
+
+val set_nth : 'a -> 'a vector -> int -> 'a -> 'a vector
