src/extraction.v
@@ -2,6 +2,7 @@
 (* (C) M. Bodin, J. Pichon - see LICENSE.txt *)
 
 From Coq Require Extraction.
+From Coq Require Import List ZArith.
 
 From Wasm Require Import
   datatypes_properties
@@ -15,9 +16,42 @@ From Wasm Require Import
   wast
 .
 
+
 From Coq Require Import
-  extraction.ExtrOcamlBasic
-  extraction.ExtrOcamlString.
+  extraction.ExtrOcamlString
+  ExtrOcamlNatBigInt
+.
+
+(* Extracting lists to (hopefully) efficient ocaml vectors using containers *)
+Extract Inductive list => "CCVector.vector"
+  [
+    "(CCVector.create ())"
+    "CCVector.push"].
+
+Extract Constant length => "Vector.length".
+Extract Constant app => "Vector.app".
+Extract Constant lookup_N => "Vector.nth_error".
+Extract Constant nth_error => "Vector.nth_error".
+Extract Constant nth => "Vector.nth".
+Extract Constant rev => "Vector.rev".
+Extract Constant in_dec => "Vector.in_dec".
+Extract Constant list_eq_dec => "Vector.vec_eq_dec".
+Extract Constant concat => "Vector.flatten".
+Extract Constant map => "Vector.map".
+Extract Constant fold_left => "Vector.fold_left".
+Extract Constant forallb => "Vector.forallb".
+Extract Constant combine => "Vector.combine".
+Extract Constant firstn => "Vector.firstn".
+Extract Constant skipn => "Vector.skipn".
+Extract Constant nodup => "Vector.nodup".
+Extract Constant repeat => "Vector.repeat".
+
+(* now dealing with ssreflect functions *)
+Extract Constant seq.size => "Vector.length".
+Extract Constant seq.cat => "Vector.app".
+Extract Constant seq.rcons => "Vector.rcons".
+Extract Constant unrcons => "Vector.unrcons".
+Extract Constant seq.set_nth => "Vector.set_nth".
 
 Extraction Language OCaml.
 
